proving most of find_entry ... really should change how seq_fund works, will ease a lot of these proofs.

examples/low-level/crypto/Crypto.AEAD.Lemmas.Part2.fst
@@ -21,6 +21,179 @@ module HS = FStar.HyperStack
 module Plain = Crypto.Plain
 module PRF = Crypto.Symmetric.PRF
 
+open Crypto.AEAD.Lemmas
+
+let prf_blocks rgn i = Seq.seq (PRF.entry rgn i)
+let aead_entries i = Seq.seq (entry i)
+
+module Cipher = Crypto.Symmetric.Cipher
+
+let find_entry (#i:id) (n:Cipher.iv (alg i)) (entries:Seq.seq (entry i)) : option (entry i) = 
+  SeqProperties.seq_find (fun e -> e.nonce = n) entries
+
+let find_entry_last (#i:id) (n:Cipher.iv (alg i)) (entries:Seq.seq (entry i){Seq.length entries > 0})
+  : Lemma (let tl, last = SeqProperties.split entries (Seq.length entries - 1) in
+	   let last = Seq.index last 0 in
+           if last.nonce = n then 
+	     find_entry n entries == Some last
+	   else find_entry n entries == find_entry n tl)
+  = let tl, last = SeqProperties.split entries (Seq.length entries - 1) in
+    let last = Seq.index last 0 in
+    if last.nonce = n then ()
+    else admit() //seq_find is annoying to work with
+
+// States consistency of the PRF table contents vs the AEAD entries
+// (not a projection from one another because of allocated MACs and aad)
+val refines_snoc: 
+  h:mem -> 
+  i:id {safeId i} -> rgn:region ->
+  entries: Seq.seq (entry i) -> 
+  blocks: Seq.seq (PRF.entry rgn i) -> GTot Type0
+  (decreases (Seq.length entries))
+let rec refines_snoc h i rgn entries blocks = 
+  if Seq.length entries = 0 then 
+    Seq.length blocks == 0 //NS:using == to get it to match with the Type returned by the other branch
+  else let entries_prefix, es = SeqProperties.split entries (Seq.length entries - 1) in
+       let e = Seq.index es 0 in
+       let b = num_blocks e in 
+       b < Seq.length blocks /\
+       (let blocks_prefix, blocks_for_e = SeqProperties.split blocks (Seq.length blocks - (b + 1)) in
+        refines_one_entry h e blocks_for_e /\
+	refines_snoc h i rgn entries_prefix blocks_prefix)
+
+
+#reset-options "--z3timeout 100 --initial_fuel 2 --max_fuel 2 --initial_ifuel 0 --max_ifuel 0"
+(* refines_one_entry can be lifted refines sums block lengths *)
+private let refines_snoc_singleton (h:mem) (i:id{safeId i}) (rgn:region) (e:entry i) (blocks_for_e:Seq.seq (PRF.entry rgn i))
+  : Lemma (requires (refines_one_entry h e blocks_for_e))
+	  (ensures (refines_snoc h i rgn (Seq.create 1 e) blocks_for_e))
+  = let b = num_blocks e in 
+    assert (Seq.equal (Seq.slice blocks_for_e (Seq.length blocks_for_e - (b + 1)) (Seq.length blocks_for_e))
+	   	      blocks_for_e)
+
+#set-options "--initial_fuel 1 --max_fuel 1 --initial_ifuel 0 --max_ifuel 0 --z3timeout 1000"
+let rec refines_snoc_append (h:mem) (i:id {safeId i}) (rgn:region)
+ 			    (entries: Seq.seq (entry i))
+			    (blocks: Seq.seq (PRF.entry rgn i))
+			    (e:entry i) (bs: Seq.seq (PRF.entry rgn i))
+       : Lemma (requires (refines_snoc h i rgn entries blocks /\
+			  refines_one_entry h e bs))
+	       (ensures  (refines_snoc h i rgn (SeqProperties.cons e entries)
+					       (Seq.append bs blocks)))
+               (decreases (Seq.length (entries)))						 
+       = if Seq.length entries = 0 then 
+	   (assert (Seq.equal (SeqProperties.cons e entries) (Seq.create 1 e));
+	    assert (Seq.equal (Seq.append bs blocks) bs);
+	    refines_snoc_singleton h i rgn e bs)
+	 else let all_entries = SeqProperties.cons e entries in
+	      let all_blocks = Seq.append bs blocks in 
+	      let all_entries_prefix, all_entries_last_es = SeqProperties.split all_entries (Seq.length all_entries - 1) in
+	      let entries_prefix, entries_last_es = SeqProperties.split entries (Seq.length entries - 1) in
+	      let last_e = Seq.index entries_last_es 0 in
+     	      assert (Seq.equal all_entries_last_es entries_last_es);
+	      let b = num_blocks last_e in 
+	      let blocks_prefix, blocks_for_last_e = SeqProperties.split blocks (Seq.length blocks - (b + 1)) in
+	      let all_blocks_prefix, all_blocks_for_last_e = SeqProperties.split all_blocks (Seq.length all_blocks - (b + 1)) in
+	      refines_snoc_append h i rgn entries_prefix blocks_prefix e bs;
+	      assert (Seq.equal all_blocks_prefix (Seq.append bs blocks_prefix));
+	      assert (Seq.equal all_entries_prefix (SeqProperties.cons e entries_prefix));
+	      assert (Seq.equal all_blocks_for_last_e blocks_for_last_e)
+
+let rec refines_refines_snoc (h:mem) (i:id {safeId i}) (rgn:region)
+ 			     (entries: Seq.seq (entry i))
+			     (blocks: Seq.seq (PRF.entry rgn i))
+     : Lemma (requires (refines h i rgn entries blocks))
+	     (ensures (refines_snoc h i rgn entries blocks))
+	     (decreases (Seq.length entries))
+     = if Seq.length entries = 0
+       then ()
+       else let hd, tl = SeqProperties.split entries 1 in 
+	    let hd = Seq.index entries 0 in
+	    let n = num_blocks hd in 
+	    let hd_blocks, blocks_tl = SeqProperties.split blocks (n + 1) in 
+	    refines_refines_snoc h i rgn tl blocks_tl;
+	    refines_snoc_append h i rgn tl blocks_tl hd hd_blocks;
+	    assert (Seq.equal entries (SeqProperties.cons hd tl));
+	    assert (Seq.equal blocks (Seq.append hd_blocks blocks_tl))
+
+#set-options "--initial_fuel 1 --max_fuel 1 --initial_ifuel 0 --max_ifuel 0 --z3timeout 100"
+val false_elim : #a:Type -> u:unit{false} -> Tot a
+let rec false_elim #a u = false_elim ()
+
+#set-options "--initial_fuel 1 --max_fuel 1 --initial_ifuel 0 --max_ifuel 0 --z3timeout 1000"
+let invert_refines_snoc (h:mem) (i:id {safeId i}) (rgn:region)
+			(entries: Seq.seq (entry i)) (blocks: Seq.seq (PRF.entry rgn i))
+   : Lemma (refines_snoc h i rgn entries blocks
+	     <==>
+	    ((Seq.length entries = 0 /\ Seq.length blocks = 0) \/ (
+	     Seq.length entries > 0 /\ (
+	     let entries_prefix, es = SeqProperties.split entries (Seq.length entries - 1) in
+	     let e = Seq.index es 0 in
+	     let b = num_blocks e in 
+	     b < Seq.length blocks /\
+	     (let blocks_prefix, blocks_for_e = SeqProperties.split blocks (Seq.length blocks - (b + 1)) in
+             refines_one_entry h e blocks_for_e /\
+	     refines_snoc h i rgn entries_prefix blocks_prefix)))))
+   = ()
+
+#reset-options "--initial_fuel 0 --max_fuel 0 --initial_ifuel 0 --max_ifuel 0 --z3timeout 1000"
+let find_blocks_append (#i:id) (#rgn:rid) (b:prf_blocks rgn i) (b':prf_blocks rgn i) (x:domain i) 
+  : Lemma (requires (is_Some (find b' x)))
+          (ensures (find (Seq.append b b') x == find b' x))
+  = admit()
+
+
+val find_entry_blocks:    (i:id) -> (rgn:rid) ->
+			  (n:Cipher.iv (alg i){safeId i}) ->
+			  (entries:aead_entries i) ->
+			  (prf_entries:prf_blocks rgn i) ->
+			  (h:mem{refines_snoc h i rgn entries prf_entries /\
+			         is_Some (find_mac prf_entries ({iv=n; ctr=ctr_0 i}))}) ->
+     Pure (entry i * prf_blocks rgn i)
+          (requires True)
+	  (ensures (fun (entry, blocks) ->
+			let x0 = {iv=n; ctr=ctr_0 i} in
+			refines_one_entry h entry blocks /\
+			find_entry n entries == Some entry /\
+			find_mac prf_entries x0 == Some (PRF.macRange rgn i x0 (Seq.index blocks 0).range)))
+	  (decreases (Seq.length entries))
+let rec find_entry_blocks i rgn n entries prf_entries h =
+  let x0 = {iv=n; ctr=ctr_0 i} in
+  let cur = Seq.length entries in 
+  invert_refines_snoc h i rgn entries prf_entries;
+  if cur = 0 
+  then false_elim()
+  else let ix = cur - 1 in 
+       let e = Seq.index entries ix in
+       let b = num_blocks e in 
+       let blocks_prefix, blocks_for_e = SeqProperties.split prf_entries (Seq.length prf_entries - (b + 1)) in
+       assert (Seq.equal prf_entries (Seq.append blocks_prefix blocks_for_e));
+       assert (refines_one_entry h e blocks_for_e);
+       let Entry nonce ad plainlen p c_tagged = e in
+       let c, tag = SeqProperties.split c_tagged plainlen in
+       let _ = find_entry_last n entries in
+       if e.nonce = n then 
+	 let _ = assert (find_entry n entries == Some e) in
+	 let hd, tl = SeqProperties.split blocks_for_e 1 in
+	 let hd = Seq.index hd 0 in
+	 assert (Seq.equal (SeqProperties.cons hd tl) blocks_for_e);
+	 let PRF.Entry x mac = hd in
+	 assert (x == x0);
+	 assert (tl == counterblocks i rgn (PRF.incr i x) plainlen 0 plainlen p c);
+	 all_above_counterblocks i rgn (PRF.incr i x) plainlen 0 plainlen p c;
+	 find_mac_counterblocks_none n tl;
+	 assert (find #rgn #i tl x0 == None);
+	 let finder (e:PRF.entry rgn i) = e.x = x0 in
+	 assume (SeqProperties.seq_find finder tl == None); //TODO: this is silly... need to investigate
+	 find_cons_hd hd tl finder;
+	 assert (find blocks_for_e x0 == Some mac);
+	 find_blocks_append blocks_prefix blocks_for_e x0;
+	 (e, blocks_for_e)
+       else let entries' = Seq.slice entries 0 (Seq.length entries - 1) in
+	    assume (find_mac prf_entries x0 == find_mac blocks_prefix x0); //TODO, need to prove that find_mac blocks_prefix x0 = None
+            find_entry_blocks i rgn n entries' blocks_prefix h
+       
+
 (*** Lemmas about modifying tables and buffers ***)
 
 let trans_all_above (#rgn:region) (#i:id) (s:Seq.seq (PRF.entry rgn i)) 
